dataplane/Examples/Ooo_Input_op.thy
@@ -1,0 +1,17 @@
+theory Ooo_Input_op
+
+imports
+  Dataplane.Timely_Stream
+  Source_op
+begin
+
+record ('p, 'd, 't) input_state = "('p, 'd, 't) operator_state" + inps:: "'p \<Rightarrow> ('t, 'd) event llist"
+
+definition ooo_input_op where
+  "ooo_input_op os = builder_op os (\<lambda> os. (cimage (\<lambda>p. case inps os p of
+    LCons (Data t d) lxs \<Rightarrow> produce (os\<lparr> inps := (inps os)(p := lxs) \<rparr>) (Cap t p) [d]
+  | LCons (Drop t) lxs \<Rightarrow> drop_cap (os\<lparr> inps := (inps os)(p := lxs) \<rparr>) (Cap t p)
+  | LCons (Mint t) lxs \<Rightarrow> mint_cap (os\<lparr> inps := (inps os)(p := lxs) \<rparr>) p t)
+    (cfilter (\<lambda>p. ocaps os p \<noteq> []) c\<UU>)))"
+
+end
